samples

Test/sequences/intseq.bpl
@@ -9,6 +9,20 @@ function {:builtin "seq.unit"} IntSeqUnit(i: int): IntSeq;
 function {:builtin "seq.nth"} IntSeqNth(s: IntSeq, i: int): int;
 function {:builtin "seq.extract"} IntSeqExtract(s: IntSeq, pos: int, len: int): IntSeq;
 
+function {:inline} IntSeqUpdate(s: IntSeq, i: int, v: int): IntSeq {
+  if (0 <= i && i < IntSeqLen(s))
+  then
+    (var s1, s2 := IntSeqExtract(s, 0, i), IntSeqExtract(s, i+1, IntSeqLen(s)-(i+1));
+     IntSeqConcat(IntSeqConcat(s1, IntSeqUnit(v)), s2))
+  else
+    s
+}
+
+function {:inline} IntSeqAppend(s:IntSeq, v: int): IntSeq {
+  IntSeqConcat(s, IntSeqUnit(v))
+}
+
+/*
 procedure test()
 {
   var s: IntSeq;
@@ -20,3 +34,75 @@ procedure test()
   assert IntSeqExtract(s, 1, 2) == IntSeqConcat(IntSeqUnit(1), IntSeqUnit(2));
   assert IntSeqNth(s, 1) == 1;
 }
+
+procedure lookup(s: IntSeq, x: int) returns (b: bool)
+ensures b == (exists i: int :: 0 <= i && i < IntSeqLen(s) && x == IntSeqNth(s, i));
+{
+  var i: int;
+
+  b := false;
+  i := 0;
+  while (i < IntSeqLen(s))
+  invariant (forall u: int :: 0 <= u && u < i ==> x != IntSeqNth(s, u));
+  invariant 0 <= i;
+  {
+    if (IntSeqNth(s, i) == x) {
+      b := true;
+      return;
+    }
+    i := i + 1;
+  }
+}
+*/
+
+function foo(s: IntSeq, x: int):int;
+
+procedure test1(s: IntSeq, x: int)
+requires 0 <= x && x < IntSeqLen(s);
+requires (forall i: int :: 0 <= i && i < IntSeqLen(s) ==> IntSeqNth(s, i) == 0);
+ensures IntSeqNth(s, x) == 0;
+{
+
+}
+
+procedure test2(s: IntSeq, x: int, y: int)
+requires 0 <= x && x <= y && y < IntSeqLen(s);
+requires (forall i, j: int :: 0 <= i && i <= j && j < IntSeqLen(s) ==> IntSeqNth(s, i) <= IntSeqNth(s, j));
+ensures IntSeqNth(s, x) <= IntSeqNth(s, y);
+{
+
+}
+
+/*
+procedure sorted_insert(s: IntSeq, x: int) returns (s': IntSeq)
+requires (forall i, j: int :: 0 <= i && i <= j && j < IntSeqLen(s) ==> IntSeqNth(s, i) <= IntSeqNth(s, j));
+ensures (forall i, j: int :: 0 <= i && i <= j && j < IntSeqLen(s) ==> IntSeqNth(s, i) <= IntSeqNth(s, j));
+{
+  var pos: int;
+  var val: int;
+
+  pos := 0;
+  while (pos < IntSeqLen(s))
+  invariant 0 <= pos;
+  invariant (forall i: int:: 0 <= i && i < pos ==> IntSeqNth(s, i) <= x);
+  {
+    if (IntSeqNth(s, pos) > x) {
+      break;
+    }
+    pos := pos + 1;
+  }
+
+  assert (forall i, j: int :: 0 <= i && i <= j && j < IntSeqLen(s) ==> IntSeqNth(s, i) <= IntSeqNth(s, j)); assume false;
+
+  val := x;
+  s' := s;
+  while (pos < IntSeqLen(s))
+  invariant 0 <= pos;
+  invariant (forall i, j: int :: 0 <= i && i <= j && j < IntSeqLen(s') ==> IntSeqNth(s', i) <= IntSeqNth(s', j));
+  {
+    s', val := IntSeqUpdate(s', pos, val), IntSeqNth(s', pos); // swap s'[pos] and val
+    pos := pos + 1;
+  }
+  s' := IntSeqAppend(s', val);
+}
+*/
